feat: structure MBA proof

SSA/Experimental/Bits/Fast/MBA.lean
@@ -3,103 +3,154 @@ theorem BitVec.zero_concat (b : Bool) : (0#0).concat b = BitVec.ofBool b := by
   apply BitVec.eq_of_getLsbD_eq
   simp
 
+@[simp]
+theorem BitVec.intCast_eq_ofInt : ((i : Int) : BitVec w) = BitVec.ofInt w i := rfl
+
+@[simp]
+theorem BitVec.intCast_zero : ((0 : Int) : BitVec w) = 0#w := by simp
+
 namespace MBA
 
 inductive Factor 
-| ofNat (x : Nat)
 | term (n : Nat)
 | and (x y : Factor) 
 | or (x y : Factor) 
 | xor (x y : Factor) 
 | not (x : Factor) 
 
-def Factor.denote (w : Nat) (xs : List (BitVec w)) : Factor → BitVec w 
-| .ofNat x => BitVec.ofNat w x
+def Env (w : Nat) := List (BitVec w)
+def Env.getLsb (env : Env w) : Env 1 := env.map <| fun x => BitVec.ofBool <| x.getLsbD 0
+def Env.getNonLsbs (env : Env w) : Env (w-1) := env.map <| fun x => x.extractLsb' 1 (w-1)
+  
+
+def Factor.reflect {w : Nat} (xs : Env w) : Factor → BitVec w 
 | .term n => xs.getD n (0#w)
-| .and x y => x.denote w xs &&& y.denote w xs
-| .or x y => x.denote w xs &&& y.denote w xs
-| .xor x y => x.denote w xs &&& y.denote w xs
-| .not x => ~~~ (x.denote w xs)
+| .and x y => x.reflect xs &&& y.reflect xs
+| .or x y => x.reflect xs ||| y.reflect xs
+| .xor x y => x.reflect xs ^^^ y.reflect xs
+| .not x => ~~~ (x.reflect xs)
+
+def Factor.denote {w : Nat} (xs : Env w) (f : Factor) : Int := f.reflect xs |>.toInt
+
+theorem Factor.reflect_eq_ofInt_denote {w : Nat} (xs : Env w) (f : Factor) : 
+    f.reflect xs = (BitVec.ofInt w <| f.denote xs) := by
+  simp [reflect, denote]
 
 @[simp]
-theorem Factor.denote_width_zero  (f : Factor) (env : List (BitVec 0)) : 
-   f.denote 0 env = 0#0 := by
+theorem Factor.reflect_zero_of_denote_zero {w : Nat} {f : Factor} {xs : Env w} (h : f.denote xs = 0) : 
+    f.reflect xs = 0#w := by
+  simp [reflect_eq_ofInt_denote, h]
+
+
+@[simp]
+theorem Factor.reflect_width_zero  (f : Factor) (env : Env 0) : 
+   f.reflect env = 0#0 := by
   apply Subsingleton.elim
 
-def Eqn := List (Int × Factor)
 
-def Eqn.denote (e : List (Int × Factor)) 
-    (w : Nat) (env : List (BitVec w)) : Int := 
+structure Term where 
+  c : Int
+  f : Factor
+
+/-- Reflect is what we use for reflection -/
+def Term.reflect {w : Nat}  (t : Term) (xs: Env w) : BitVec w := 
+  t.c * t.f.reflect xs 
+
+def Term.denote {w : Nat} (t : Term) (xs : Env w) : Int := 
+  t.c * t.f.denote xs
+
+
+@[simp]
+theorem Term.reflect_eq_ofInt_denote {w : Nat} {t : Term} {xs : Env w} :
+    t.reflect xs = (BitVec.ofInt w <| t.denote xs) := by
+  obtain ⟨c, f⟩ := t 
+  simp [Term.reflect, Term.denote]
+  rw [BitVec.ofInt_mul]
+  rw [Factor.reflect_eq_ofInt_denote]
+
+@[simp]
+theorem Term.reflect_zero_of_denote_zero {w : Nat} {t : Term} {xs : Env w} (h : t.denote xs = 0) : 
+    t.reflect xs = 0#w := by
+  simp [Term.reflect_eq_ofInt_denote, h]
+
+@[simp]
+theorem Term.reflect_width_zero  (t : Term) (env : Env 0) : 
+    t.reflect env = 0 := by simp [Term.reflect]
+
+def Eqn := List Term
+
+def Eqn.reflect {w : Nat} (e : Eqn) (env : Env w) : BitVec w := 
   match e with
   | [] => 0
-  | (coeff, x) :: xs => coeff * (x.denote w env).toInt + Eqn.denote xs w env 
+  | t :: ts => t.reflect env + Eqn.reflect ts env
 
 @[simp]
-theorem Eqn.denote_nil  (w : Nat) (env : List (BitVec w)) : 
-    Eqn.denote [] w env = 0 := rfl
+theorem Eqn.reflect_nil  {w : Nat} (env : Env w) : 
+    Eqn.reflect [] env = 0 := rfl
 
 @[simp]
-theorem Eqn.denote_cons
-    (coeff : Int) (x : Factor) (es : List (Int × Factor)) (w : Nat) (env : List (BitVec w)) : 
-    Eqn.denote ((coeff, x) :: es) w env = coeff * (x.denote w env).toInt + Eqn.denote es w env := rfl
+theorem Eqn.reflect_cons {w : Nat}
+    (t : Term) (ts : List Term) (env : Env w) : 
+    Eqn.reflect (t :: ts) env = t.reflect env + Eqn.reflect ts env := rfl
+
+
+def Eqn.denote {w : Nat} (e : Eqn) (env : Env w) : Int := 
+  match e with
+  | [] => 0
+  | t :: ts => t.denote env + Eqn.denote ts env
 
 @[simp]
-theorem Eqn.denote_width_zero  (es : List (Int × Factor)) (env : List (BitVec 0)) : 
-    Eqn.denote es 0 env = 0 := by 
+theorem Eqn.denote_nil  {w : Nat} (env : Env w) : 
+    Eqn.denote [] env = 0 := rfl
+
+@[simp]
+theorem Eqn.denote_cons {w : Nat}
+    (t : Term) (ts : List Term) (env : Env w) : 
+    Eqn.denote (t :: ts) env = t.denote env + Eqn.denote ts env := rfl
+
+@[simp]
+theorem Eqn.reflect_width_zero  (es : Eqn) (env : Env 0) : 
+    Eqn.reflect es env = 0 := by 
   induction es 
-  case nil => simp [Eqn.denote]
+  case nil => simp [Eqn.reflect]
   case cons e es ih => 
-    obtain ⟨c, f⟩ := e
-    simp [ih]
-
-/-
-@[simp]
-theorem Eqn.denote_cons'
-    (e : Int × Factor) (es : List (Int × Factor)) (w : Nat) (env : List (BitVec w)) : 
-    Eqn.denote (e :: es) w env = e.1 * (e.2.denote w env) + Eqn.denote es w env := rfl
+    simp [ih, Eqn.reflect]
+    apply Subsingleton.elim
 
 @[simp]
-theorem Eqn.denote_zero (e : List (Int × Factor)) (env : List (BitVec 0)) : 
-    Eqn.denote e 0 env = 0#0 := by 
-  apply Subsingleton.elim
--/
+theorem Eqn.reflect_eq_ofInt_denote {w : Nat} (xs : Env w) (e : Eqn) :
+    e.reflect xs = BitVec.ofInt w (e.denote xs) := by
+  induction e 
+  case nil => simp 
+  case cons t ts ih => 
+    simp 
+    simp [BitVec.ofInt_add, ih]
 
-theorem Eqn.denote_succ (e : Eqn) (w : Nat) (env : List (BitVec (w + 1))) : 
-    Eqn.denote e (w + 1) env = 
-      2 * (Eqn.denote e w (env.map <| fun x => x.extractLsb' 1 w)) +
-      (Eqn.denote e 1 (env.map <| fun x => BitVec.ofBool <| x.getLsbD 0)) := by
-  induction w
-  case zero => 
-    simp
-    induction e 
-    case nil => simp
-    case cons e es ih =>
-      obtain ⟨coeff, f⟩ := e
-      simp
-      rw [← ih]
-      congr
-      suffices heq : (fun x => BitVec.ofBool (x.getLsbD 0)) = id by simp [heq]
-      ext x i hi
-      have : i = 0 := by omega
-      simp [this]
-  case succ w ih =>
-    sorry
-    
 
-theorem Eqn.denote_hard_case (e : Eqn) (h : ∀ (env : List (BitVec 1)), Eqn.denote e 1 env = 0) :
-    ∀ (w : Nat) (env : List (BitVec w)), Eqn.denote e w env = 0 := by
+@[simp]
+theorem Eqn.reflect_zero_of_denote_zero {w : Nat} (xs : Env w) (e : Eqn) (h : e.denote xs = 0) :
+    e.reflect xs = 0 := by simp [h]
+
+@[simp]
+def Env.getLsb_eq_of_width_one (env : List (BitVec 1)) : Env.getLsb env = env := by
+  simp [getLsb]
+  suffices heq : (fun x => BitVec.ofBool (x.getLsbD 0)) = id by simp [heq]
+  ext x i hi
+  have : i = 0 := by omega
+  simp [this]
+  
+      
+theorem Eqn.denote_hard_case (e : Eqn) (h : ∀ (env1 : List (BitVec 1)), Eqn.reflect e env1 = 0) :
+    ∀ {w : Nat} (env : List (BitVec w)), e.reflect env = 0 := by
   intros w env 
   induction w 
   case zero => simp
   case succ w ih =>
-    rw [Eqn.denote_succ]
-    rw [h]
-    rw [ih]
-    simp
+    sorry
 
 theorem Eqn.denote_iff_denote_one (e : Eqn) : 
-    (∀ (w : Nat) (env : List (BitVec w)), Eqn.denote e w env = 0) ↔ 
-    (∀ env : List (BitVec 1), Eqn.denote e 1 env = 0) := by
+    (∀ (w : Nat) (env : List (BitVec w)), Eqn.reflect e env = 0) ↔ 
+    (∀ env1 : List (BitVec 1), Eqn.reflect e env1 = 0) := by
   constructor 
   · intros h
     apply h
